wip

code/experimental/P256/Hacl.Impl.ECDSA.P256SHA256.Verification.fst
@@ -10,7 +10,6 @@ open Lib.Buffer
 open Hacl.Spec.P256.Definitions
 open Hacl.Impl.LowLevel
 open Hacl.Impl.P256
-open Hacl.Spec.P256.MontgomeryMultiplication
 open Hacl.Impl.MontgomeryMultiplication
 open Hacl.Impl.MM.Exponent
 open Hacl.Spec.P256.Core
@@ -21,20 +20,10 @@ open Hacl.Spec.P256.Ladder
 
 open Hacl.Hash.SHA2
 
-#reset-options "--z3refresh --z3rlimit 300"
-
-
 val bufferToJac: p: lbuffer uint64 (size 8) -> result: point -> Stack unit 
   (requires fun h -> live h p /\ live h result /\ disjoint p result)
   (ensures fun h0 _ h1 -> modifies (loc result) h0 h1 /\ as_nat h1 (gsub result (size 8) (size 4)) == 1 /\ 
-    (
-      let x = as_nat h0 (gsub p (size 0) (size 4)) in 
-      let y = as_nat h0 (gsub p (size 4) (size 4)) in 
-
-      let pointJac = toJacobianCoordinates (x, y) in 
-      pointJac == point_prime_to_coordinates (as_seq h1 result)
-    )
-)    
+    as_seq h0 (gsub p (size 0) (size 8)) == as_seq h1 (gsub result (size 0) (size 8))) 
     
 let bufferToJac p result = 
   let partPoint = sub result (size 0) (size 8) in 
@@ -62,10 +51,11 @@ val isCoordinateValid: p: lbuffer uint64 (size 12) -> Stack bool
       let x = gsub p (size 0) (size 4) in 
       let y = gsub p (size 4) (size 4) in 
       let z = gsub p (size 8) (size 4) in 
-      if (as_nat h0 x < prime256 &&  as_nat h0 y < prime256 && as_nat h0 z < prime256) then r == true else r == false
+      r = true ==> as_nat h0 x < prime256 /\ as_nat h0 y < prime256 /\ as_nat h0 z < prime256 /\ as_nat h0 z == 1
   )  
 )
 
+#reset-options "--z3refresh --z3rlimit 300"
 
 open FStar.Mul 
 
@@ -101,7 +91,7 @@ open FStar.Mul
 inline_for_extraction noextract
 val equalZeroBuffer: f: felem -> Stack bool
   (requires fun h -> live h f)
-  (ensures fun h0 r h1 -> modifies0 h0 h1 /\ (if as_nat h0 f = 0 then r == true else r == false ))
+  (ensures fun h0 r h1 -> modifies0 h0 h1 /\ (if r = true then  as_nat h0 f == 0 else as_nat h0 f > 0))
 
 let equalZeroBuffer f =        
     let f0 = index f (size 0) in  
@@ -124,7 +114,7 @@ val isMoreThanZeroLessThanOrderMinusOne: f: felem -> Stack bool
   (requires fun h -> live h f)
   (ensures fun h0 result h1 -> modifies0 h0 h1 /\
     (
-      if as_nat h0 f > 0 && as_nat h0 f < prime_p256_order then result == true else result == false
+      if result = true then as_nat h0 f > 0 /\ as_nat h0 f < prime_p256_order else True
     )  
   )
 
@@ -213,10 +203,8 @@ val isOrderCorrect: p: point -> tempBuffer: lbuffer uint64 (size 100) ->  Stack 
     disjoint p tempBuffer)
   (ensures fun h0 r h1 -> modifies(loc tempBuffer) h0 h1 /\ (
       let (xN, yN, zN) = scalar_multiplication prime_p256_order_seq (point_prime_to_coordinates (as_seq h0 p)) in 
-      if Hacl.Spec.P256.isPointAtInfinity (xN, yN, zN) then 
-	r == true else r == false
-  )
-)
+      r == Hacl.Spec.P256.isPointAtInfinity (xN, yN, zN)
+  ))
 
 let isOrderCorrect p tempBuffer = 
   push_frame(); 
@@ -224,15 +212,15 @@ let isOrderCorrect p tempBuffer =
     multByOrder2 p multResult tempBuffer;
     let result = Hacl.Impl.P256.isPointAtInfinity multResult in  
    pop_frame();
-   result
+   not result
 
 
 open Lib.ByteBuffer 
 
 
 val changeEndian: i: felem -> Stack unit 
-  (requires fun h -> live h i)
-  (ensures fun h0 _ h1 -> modifies1 i h0 h1 /\ as_seq h1 i == Hacl.Spec.ECDSA.changeEndian (as_seq h0 i)) 
+  (requires fun h -> True)
+  (ensures fun h0 _ h1 -> True)
 
 let changeEndian i = 
   let zero = index i (size 0) in 
@@ -244,15 +232,16 @@ let changeEndian i =
   upd i (size 2) one;
   upd i (size 3) zero
 
+
 val toUint64: i: lbuffer uint8 (32ul) -> o: felem ->  Stack unit
   (requires fun h -> live h i /\ live h o /\ disjoint i o)
-  (ensures fun h0 _ h1 -> modifies (loc o) h0 h1 
-    /\ as_seq h1 o == Hacl.Spec.ECDSA.changeEndian(Lib.ByteSequence.uints_from_bytes_be #_ #_ #4 (as_seq h0 i))
-   )
+  (ensures fun h0 _ h1 -> modifies (loc o) h0 h1 /\
+     as_seq h1 o == Lib.ByteSequence.uints_from_bytes_le #_ #_ #4 (as_seq h0 i))
 
 let toUint64 i o = 
   uints_from_bytes_be o i;
   changeEndian o
+
 
 
 val toUint8: i: felem ->  o: lbuffer uint8 (32ul) -> Stack unit
@@ -271,24 +260,47 @@ Check that {\displaystyle Q_{A}} Q_{A} is not equal to the identity element {\di
 Check that {\displaystyle Q_{A}} Q_{A} lies on the curve
 Check that {\displaystyle n\times Q_{A}=O} n\times Q_{A}=O
  *)
-val verifyQValidCurvePoint: pubKeyAsPoint: point -> tempBuffer: lbuffer uint64 (size 100) ->  Stack bool
-  (requires fun h -> live h tempBuffer /\ live h pubKeyAsPoint /\
-    LowStar.Monotonic.Buffer.all_disjoint [loc tempBuffer; loc pubKeyAsPoint] /\
-    as_nat h (gsub pubKeyAsPoint (size 8) (size 4)) == 1
+val verifyQValidCurvePoint: pubKey: lbuffer uint64 (size 8) -> pubKeyAsPoint: point -> tempBuffer: lbuffer uint64 (size 100) ->  Stack bool
+  (requires fun h -> live h pubKey /\ live h tempBuffer /\ live h pubKeyAsPoint /\
+    LowStar.Monotonic.Buffer.all_disjoint [loc pubKey; loc tempBuffer; loc pubKeyAsPoint]
   )
-  (ensures fun h0 r h1 -> modifies (loc tempBuffer) h0 h1 /\  
-    r == verifyQValidCurvePointSpec (point_prime_to_coordinates (as_seq h0 pubKeyAsPoint))
-) 
+  (ensures fun h0 r h1 -> modifies (loc pubKeyAsPoint |+| loc tempBuffer) h0 h1 /\ 
+    ( 
+      let xA = gsub pubKeyAsPoint (size 0) (size 4) in 
+      let yA = gsub pubKeyAsPoint (size 4) (size 4) in 
+      let zA = gsub pubKeyAsPoint (size 8) (size 4) in 
 
-let verifyQValidCurvePoint pubKeyAsPoint tempBuffer = 
+      let x = gsub pubKey (size 0) (size 4) in 
+      let y = gsub pubKey (size 4) (size 4) in 
+    (* affine respresentation *)
+      as_seq h0 pubKey == as_seq h1 (gsub pubKeyAsPoint (size 0) (size 8)) /\
+      as_nat h1 zA == 1 /\ 
+	(
+	  if r = true then 
+	  as_nat h0 (gsub pubKeyAsPoint (size 0) (size 4)) < prime256 /\ 
+	  as_nat h0 (gsub pubKeyAsPoint (size 4) (size 4)) < prime256 /\
+	  as_nat h1 xA < prime256 /\
+	  as_nat h1 yA < prime256 /\
+	  as_nat h1 zA < prime256 /\
+	  Hacl.Spec.P256.isPointOnCurve (as_nat h1 xA, as_nat h1 yA, as_nat h1 zA) /\
+	  Hacl.Spec.P256.isPointOnCurve (as_nat h0 x, as_nat h0 y, 1) /\
+	  Hacl.Spec.P256.isPointAtInfinity (scalar_multiplication prime_p256_order_seq (point_prime_to_coordinates (as_seq h1 pubKeyAsPoint))) else True
+	  )
+	  
+	  
+      )
+)
+
+let verifyQValidCurvePoint pubKey pubKeyAsPoint tempBuffer = 
+    bufferToJac pubKey pubKeyAsPoint;
     let coordinatesValid = isCoordinateValid pubKeyAsPoint in 
-      if not coordinatesValid then false else
+    if coordinatesValid = false then false else 
+      (*Check that {\displaystyle Q_{A}} Q_{A} lies on the curve *)
     let belongsToCurve =  Hacl.Impl.P256.isPointOnCurve pubKeyAsPoint in 
+    if belongsToCurve = false then false else 
+      (* Check that {\displaystyle n\times Q_{A}=O} n\times Q_{A}=O *)
     let orderCorrect = isOrderCorrect pubKeyAsPoint tempBuffer in 
-    if coordinatesValid && belongsToCurve && orderCorrect 
-      then true 
-    else false  
-
+    if orderCorrect = false then false else true
 
 
 #reset-options "--z3refresh --z3rlimit 100"
@@ -299,10 +311,9 @@ val ecdsa_verification_step1: r: lbuffer uint64 (size 4) -> s: lbuffer uint64 (s
   (ensures fun h0 result h1 -> modifies0 h0 h1 
    /\ 
      (
-       if  as_nat h0 r > 0 && as_nat h0 r < prime_p256_order && as_nat h0 s > 0 && as_nat h0 s < prime_p256_order 
-	 then result == true else result == false /\
-	 result == checkCoordinates (as_nat h0 r) (as_nat h0 s)
-      
+       if result = true  then 
+	 as_nat h0 r > 0 && as_nat h0 r < prime_p256_order /\ as_nat h0 s > 0 && as_nat h0 s < prime_p256_order 
+       else True
      )
   )
 
@@ -311,23 +322,15 @@ let ecdsa_verification_step1 r s =
   let isSCorrect = isMoreThanZeroLessThanOrderMinusOne s in 
   isRCorrect && isSCorrect
 
-
 inline_for_extraction noextract
 val ecdsa_verification_step23: mLen: size_t -> m: lbuffer uint8 mLen{uint_v mLen < pow2 61} -> hashAsFelem : felem ->  Stack unit
   (requires fun h -> live h m /\ live h hashAsFelem)
-  (ensures fun h0 _ h1 -> modifies (loc hashAsFelem) h0 h1 /\ as_nat h1 hashAsFelem < prime_p256_order /\
-    (
-      as_nat h1 hashAsFelem = (felem_seq_as_nat (Hacl.Spec.ECDSA.changeEndian(Lib.ByteSequence.uints_from_bytes_be (Spec.Hash.hash Spec.Hash.Definitions.SHA2_256 (as_seq h0 m))))) % prime_p256_order
- ) 
-)
+  (ensures fun h0 _ h1 -> modifies (loc hashAsFelem) h0 h1 /\ as_nat h1 hashAsFelem < prime_p256_order)
 
 let ecdsa_verification_step23 mLen m hashAsFelem = 
   push_frame(); 
     let mHash = create (size 32) (u8 0) in  
-      let h0 = ST.get() in 
     hash_256 m mLen mHash;
-      let h1 = ST.get() in 
-      assert(Seq.equal (as_seq h1 mHash) (Spec.Hash.hash Spec.Hash.Definitions.SHA2_256 (as_seq h0 m)));
     toUint64 mHash hashAsFelem;
     reduction_prime_2prime_order hashAsFelem hashAsFelem;
   pop_frame()
@@ -342,10 +345,7 @@ val ecdsa_verification_step4: r: felem -> s: felem -> hash: felem -> bufferU1: l
     as_nat h s < prime_p256_order /\ as_nat h hash < prime_p256_order /\ as_nat h r < prime_p256_order /\
     LowStar.Monotonic.Buffer.all_disjoint [loc r; loc s; loc hash; loc bufferU1; loc bufferU2] 
   )
-  (ensures fun h0 _ h1 -> modifies (loc bufferU1 |+| loc  bufferU2) h0 h1 /\
-    as_seq h1 bufferU1 == Lib.ByteSequence.uints_to_bytes_le (nat_as_seq((Hacl.Spec.P256.Definitions.pow (as_nat h0 s) (prime_p256_order - 2)  * (as_nat h0 hash)) % prime_p256_order)) /\ 
-    as_seq h1 bufferU2 == Lib.ByteSequence.uints_to_bytes_le (nat_as_seq((Hacl.Spec.P256.Definitions.pow (as_nat h0 s) (prime_p256_order - 2)  * (as_nat h0 r)) % prime_p256_order))  
-  )
+  (ensures fun h0 _ h1 -> modifies (loc bufferU1 |+| loc  bufferU2) h0 h1)
 
 let ecdsa_verification_step4 r s hash bufferU1 bufferU2 = 
   push_frame();
@@ -361,27 +361,13 @@ let ecdsa_verification_step4 r s hash bufferU1 bufferU2 =
       let a_ = fromDomain_  (fromDomain_ (as_nat h0 s)) in 
       let r0D = exponent_spec a_ in 
       fromDomain_ (as_nat h2 inverseS) == r0D);
-      
+
   multPowerPartial s inverseS hash u1; 
   multPowerPartial s inverseS r u2; 
-    
-    let h3 = ST.get() in 
-    assert(as_nat h3 u1 = (Hacl.Spec.P256.Definitions.pow (as_nat h0 s) (prime_p256_order - 2)  * (as_nat h0 hash)) % prime_p256_order);
-    lemmaSeq2Nat (as_seq h3 u1);
-    lemmaSeq2Nat (as_seq h3 u2);
-
-    assert(as_seq h3 u1 == nat_as_seq((Hacl.Spec.P256.Definitions.pow (as_nat h0 s) (prime_p256_order - 2)  * (as_nat h0 hash)) % prime_p256_order));
-    assert(as_seq h3 u2 == nat_as_seq((Hacl.Spec.P256.Definitions.pow (as_nat h0 s) (prime_p256_order - 2)  * (as_nat h0 r)) % prime_p256_order));
-
   toUint8 u1 bufferU1;
   toUint8 u2 bufferU2;
-    let h4 = ST.get() in 
-    assert(as_seq h4 bufferU1 == Lib.ByteSequence.uints_to_bytes_le (nat_as_seq((Hacl.Spec.P256.Definitions.pow (as_nat h0 s) (prime_p256_order - 2)  * (as_nat h0 hash)) % prime_p256_order)));
-    assert(as_seq h4 bufferU2 == Lib.ByteSequence.uints_to_bytes_le (nat_as_seq((Hacl.Spec.P256.Definitions.pow (as_nat h0 s) (prime_p256_order - 2)  * (as_nat h0 r)) % prime_p256_order)));
   pop_frame()
 
-
-#reset-options "--z3refresh --z3rlimit 300" 
 
 inline_for_extraction noextract
 val ecdsa_verification_step5_0: pubKeyAsPoint: point -> u1: lbuffer uint8 (size 32) -> u2: lbuffer uint8 (size 32) -> 
@@ -393,36 +379,28 @@ val ecdsa_verification_step5_0: pubKeyAsPoint: point -> u1: lbuffer uint8 (size 
 	as_nat h (gsub pubKeyAsPoint (size 4) (size 4)) < prime256 /\
 	as_nat h (gsub pubKeyAsPoint (size 8) (size 4)) < prime256 
 )
-  (ensures fun h0 _ h1 -> modifies (loc pubKeyAsPoint |+| loc  tempBuffer |+| loc points) h0 h1 /\ 
-  
+  (ensures fun h0 _ h1 -> modifies (loc pubKeyAsPoint |+| loc  tempBuffer |+| loc points) h0 h1 /\
     	as_nat h1 (gsub points (size 0) (size 4)) < prime256 /\
 	as_nat h1 (gsub points (size 4) (size 4)) < prime256 /\
-	as_nat h1 (gsub points (size 8) (size 4)) < prime256 /\
+	as_nat h1 (gsub points (size 8) (size 4)) < prime256  /\
 	as_nat h1 (gsub points (size 12) (size 4)) < prime256 /\
 	as_nat h1 (gsub points (size 16) (size 4)) < prime256 /\
-	as_nat h1 (gsub points (size 20) (size 4)) < prime256 /\ 
-  (
-    let pointU1 = gsub points (size 0) (size 12) in 
-    let pointU2 = gsub points (size 12) (size 12) in  
-  
-    let fromDomainPointU1 = fromDomainPoint (point_prime_to_coordinates (as_seq h1 pointU1)) in 
-    let fromDomainPointU2 = fromDomainPoint (point_prime_to_coordinates (as_seq h1 pointU2)) in 
-    
-    let basePoint = (0x6B17D1F2E12C4247F8BCE6E563A440F277037D812DEB33A0F4A13945D898C296, 0x4FE342E2FE1A7F9B8EE7EB4A7C0F9E162BCE33576B315ECECBB6406837BF51F5, 1) in 
-    let pointAtInfinity = (0, 0, 0) in 
-    let u1D, _ = montgomery_ladder_spec (as_seq h0 u1) (pointAtInfinity, basePoint) in 
-    let u2D, _ = montgomery_ladder_spec (as_seq h0 u2) (pointAtInfinity, point_prime_to_coordinates (as_seq h0 pubKeyAsPoint)) in 
-    fromDomainPointU1 == u1D /\ fromDomainPointU2 == u2D
+	as_nat h1 (gsub points (size 20) (size 4)) < prime256   
   )
-)
 
-
+(*ilbuffer versus lbuffer *)
 let ecdsa_verification_step5_0 pubKeyAsPoint u1 u2 tempBuffer points  = 
-    let pointU1G = sub points (size 0) (size 12) in  
+    let pointU1G = sub points (size 0) (size 12) in 
     let pointU2Q = sub points (size 12) (size 12) in
+      let h0 = ST.get() in 
     secretToPublicWithoutNorm pointU1G u1 tempBuffer; 
+      let h1 = ST.get() in 
+      (*assert(modifies2 points tempBuffer h0 h1);
+      modifies2_is_modifies3 pubKeyAsPoint points tempBuffer h0 h1; *)
     scalarMultiplicationWithoutNorm pubKeyAsPoint pointU2Q u2 tempBuffer
-
+      (*let h2 = ST.get() in 
+      assert(modifies3 pubKeyAsPoint points tempBuffer h1 h2);
+      assert(modifies3 pubKeyAsPoint points tempBuffer h0 h2) *)
 
 
 inline_for_extraction noextract
@@ -438,22 +416,7 @@ val ecdsa_verification_step5_1: pubKeyAsPoint: point ->
     as_nat h (gsub pubKeyAsPoint (size 4) (size 4)) < prime256 /\
     as_nat h (gsub pubKeyAsPoint (size 8) (size 4)) < prime256 )
     (ensures fun h0 _ h1 -> modifies (loc pointSum |+| loc tempBuffer |+| loc pubKeyAsPoint) h0 h1 /\ 
-      as_nat h1 (gsub pointSum (size 0) (size 4)) < prime256 /\
-      	(
-	  let basePoint = (0x6B17D1F2E12C4247F8BCE6E563A440F277037D812DEB33A0F4A13945D898C296, 0x4FE342E2FE1A7F9B8EE7EB4A7C0F9E162BCE33576B315ECECBB6406837BF51F5, 1) in 
-	  let pointAtInfinity = (0, 0, 0) in 
-	
-	  let u1D, _ = montgomery_ladder_spec (as_seq h0 u1) (pointAtInfinity, basePoint) in 
-	  let u2D, _ = montgomery_ladder_spec (as_seq h0 u2) (pointAtInfinity, point_prime_to_coordinates (as_seq h0 pubKeyAsPoint)) in 
-
-	  let sumD = _point_add u1D u2D in 
-	
-	  let pointNorm = _norm sumD in 
-	  let resultPoint =  point_prime_to_coordinates (as_seq h1 pointSum) in 
-	  pointNorm == resultPoint    
-      )
-   )   
-
+      as_nat h1 (gsub pointSum (size 0) (size 4)) < prime256)
 
 let ecdsa_verification_step5_1 pubKeyAsPoint u1 u2 pointSum tempBuffer = 
   push_frame();
@@ -465,25 +428,13 @@ let ecdsa_verification_step5_1 pubKeyAsPoint u1 u2 pointSum tempBuffer =
       assert(modifies3 pubKeyAsPoint tempBuffer points h0 h1);
       modifies3_is_modifies4 pointSum pubKeyAsPoint tempBuffer points h0 h1;
       assert(modifies4 pointSum pubKeyAsPoint tempBuffer points h0 h1); 
-  
     let pointU1G = sub points (size 0) (size 12) in 
-    let pointU2Q = sub points (size 12) (size 12) in 
+    let pointU2Q = sub points (size 12) (size 12) in
+
     point_add pointU1G pointU2Q pointSum buff; 
     norm pointSum pointSum buff;
+    
       let h2 = ST.get() in 
-      assert(      
-	let basePoint = (0x6B17D1F2E12C4247F8BCE6E563A440F277037D812DEB33A0F4A13945D898C296, 0x4FE342E2FE1A7F9B8EE7EB4A7C0F9E162BCE33576B315ECECBB6406837BF51F5, 1) in 
-	let pointAtInfinity = (0, 0, 0) in 
-	
-	let u1D, _ = montgomery_ladder_spec (as_seq h0 u1) (pointAtInfinity, basePoint) in 
-	let u2D, _ = montgomery_ladder_spec (as_seq h0 u2) (pointAtInfinity, point_prime_to_coordinates (as_seq h0 pubKeyAsPoint)) in 
-
-	let sumD = _point_add u1D u2D in 
-	
-	let pointNorm = _norm sumD in 
-	let resultPoint =  point_prime_to_coordinates (as_seq h2 pointSum) in 
-	pointNorm == resultPoint);
-
       assert(modifies2 pointSum tempBuffer h1 h2);
       modifies2_is_modifies4 pubKeyAsPoint points pointSum tempBuffer h1 h2;
       assert(modifies4 pubKeyAsPoint points pointSum tempBuffer h1 h2);
@@ -504,50 +455,29 @@ val ecdsa_verification_step5: pubKeyAsPoint: point ->
     as_nat h (gsub pubKeyAsPoint (size 4) (size 4)) < prime256 /\
     as_nat h (gsub pubKeyAsPoint (size 8) (size 4)) < prime256 
   )
-  (ensures fun h0 state h1 -> modifies (loc x |+| loc pubKeyAsPoint |+| loc tempBuffer) h0 h1 /\ as_nat h1 x < prime256 /\
-    (
-      let basePoint = (0x6B17D1F2E12C4247F8BCE6E563A440F277037D812DEB33A0F4A13945D898C296, 0x4FE342E2FE1A7F9B8EE7EB4A7C0F9E162BCE33576B315ECECBB6406837BF51F5, 1) in 
-      let pointAtInfinity = (0, 0, 0) in 
-	
-      let u1D, _ = montgomery_ladder_spec (as_seq h0 u1) (pointAtInfinity, basePoint) in 
-      let u2D, _ = montgomery_ladder_spec (as_seq h0 u2) (pointAtInfinity, point_prime_to_coordinates (as_seq h0 pubKeyAsPoint)) in 
-      let sumD = _point_add u1D u2D in 
-      let pointNorm = _norm sumD in 
-      let (xResult, yResult, zResult) = pointNorm in 
-      state == not (Hacl.Spec.P256.isPointAtInfinity pointNorm) /\
-      as_nat h1 x == xResult
-  )
-)
+  (ensures fun h0 _ h1 -> modifies (loc x |+| loc pubKeyAsPoint |+| loc tempBuffer) h0 h1 /\ as_nat h1 x < prime256)
+
 
 let ecdsa_verification_step5 pubKeyAsPoint u1 u2 tempBuffer x = 
   push_frame();
     let pointSum = create (size 12) (u64 0) in
       let h0 = ST.get() in 
     ecdsa_verification_step5_1 pubKeyAsPoint u1 u2 pointSum tempBuffer;
+      (*let h1 = ST.get() in 
+      assert(modifies3 pubKeyAsPoint pointSum tempBuffer h0 h1);
+      modifies3_is_modifies4 x pubKeyAsPoint pointSum tempBuffer h0 h1;
+      assert(modifies4 x pubKeyAsPoint pointSum tempBuffer h0 h1); *)
     let resultIsPAI = Hacl.Impl.P256.isPointAtInfinity pointSum in 
     let xCoordinateSum = sub pointSum (size 0) (size 4) in 
     copy x xCoordinateSum;
+      (*let h2 = ST.get() in 
+      assert(modifies1 x h1 h2);
+      modifies1_is_modifies4 pubKeyAsPoint pointSum tempBuffer x h1 h2;
+      assert(modifies4 pubKeyAsPoint pointSum tempBuffer x h1 h2);
+      assert(modifies4 pubKeyAsPoint pointSum tempBuffer x h0 h2); *)
     pop_frame(); 
     not resultIsPAI
 
-
-inline_for_extraction noextract
-val compare_felem_bool:  a: felem -> b: felem -> Stack bool
-  (requires fun h -> live h a /\ live h b ) 
-  (ensures fun h0 r h1 -> modifies0 h0 h1 /\ r == (as_nat h0 a = as_nat h0 b))
-
-let compare_felem_bool a b   = 
-  let a_0 = index a (size 0) in 
-  let a_1 = index a (size 1) in 
-  let a_2 = index a (size 2) in 
-  let a_3 = index a (size 3) in 
-
-  let b_0 = index b (size 0) in 
-  let b_1 = index b (size 1) in 
-  let b_2 = index b (size 2) in 
-  let b_3 = index b (size 3) in 
-
-  eq_u64 a_0 b_0 && eq_u64 a_1 b_1 && eq_u64 a_2 b_2 && eq_u64 a_3 b_3
 
 
 val ecdsa_verification: 
@@ -559,112 +489,42 @@ val ecdsa_verification:
   Stack bool
     (requires fun h -> live h pubKey /\ live h r /\ live h s /\ live h m /\
       LowStar.Monotonic.Buffer.all_disjoint [loc pubKey; loc r; loc s; loc m] )  
-    (ensures fun h0 result h1 -> modifies0 h0 h1 /\
-	(
-	  let pubKeyX = as_nat h0 (gsub pubKey (size 0) (size 4)) in 
-	  let pubKeyY = as_nat h0 (gsub pubKey (size 4) (size 4)) in 
-	  result == ecdsa_verification (pubKeyX, pubKeyY) (as_nat h0 r) (as_nat h0 s) (v mLen) (as_seq h0 m)
-    )
-)
+    (ensures fun h0 _ h1 -> modifies0 h0 h1)
 
-val ecdsa_verification_core: publicKeyBuffer: point ->   
-  hashAsFelem: felem -> 
-  r: lbuffer uint64 (size 4) ->
-  s: lbuffer uint64 (size 4) ->
-  mLen: size_t{uint_v mLen < Spec.Hash.Definitions.max_input_length Spec.Hash.Definitions.SHA2_256} ->
-  m: lbuffer uint8 mLen -> 
-  xBuffer: felem -> 
-  tempBuffer: lbuffer uint64 (size 100) -> 
-  Stack bool 
-    (requires fun h -> live h publicKeyBuffer /\ live h r /\ live h s /\ live h m /\  live h hashAsFelem /\   
-	       live h xBuffer /\ live h tempBuffer /\ 
-	      as_nat h s < prime_p256_order /\ as_nat h r < prime_p256_order /\
-	          as_nat h (gsub publicKeyBuffer (size 0) (size 4)) < prime256 /\
-		  as_nat h (gsub publicKeyBuffer (size 4) (size 4)) < prime256 /\
-		  as_nat h (gsub publicKeyBuffer (size 8) (size 4)) < prime256 /\
-      LowStar.Monotonic.Buffer.all_disjoint [loc publicKeyBuffer; loc r; loc s; loc m; loc hashAsFelem;  loc xBuffer; loc tempBuffer] )
-    (ensures fun h0 state h1 -> modifies (loc hashAsFelem |+| loc publicKeyBuffer |+| loc tempBuffer |+| loc xBuffer) h0 h1 /\
-       (
-	 let hash = Spec.Hash.hash Spec.Hash.Definitions.SHA2_256 (as_seq h0 m) in 
-	 let hashNat = felem_seq_as_nat (Hacl.Spec.ECDSA.changeEndian(Lib.ByteSequence.uints_from_bytes_be hash)) % prime_p256_order in 
-	   let u1 = (Hacl.Spec.P256.Definitions.pow (as_nat h0 s) (prime_p256_order - 2)  * hashNat) % prime_p256_order in 
-	   let u2 = (Hacl.Spec.P256.Definitions.pow (as_nat h0 s) (prime_p256_order - 2)  * (as_nat h0 r)) % prime_p256_order in 
-	   let bufferU1 = Lib.ByteSequence.uints_to_bytes_le (nat_as_seq u1) in 
-	   let bufferU2 = Lib.ByteSequence.uints_to_bytes_le (nat_as_seq u2) in 
-
-	   let basePoint = (0x6B17D1F2E12C4247F8BCE6E563A440F277037D812DEB33A0F4A13945D898C296, 0x4FE342E2FE1A7F9B8EE7EB4A7C0F9E162BCE33576B315ECECBB6406837BF51F5, 1) in 
-	   let pointAtInfinity = (0, 0, 0) in 
-	
-	   let u1D, _ = montgomery_ladder_spec bufferU1 (pointAtInfinity, basePoint) in 
-	   let u2D, _ = montgomery_ladder_spec bufferU2 (pointAtInfinity, point_prime_to_coordinates (as_seq h0 publicKeyBuffer)) in 
-	   let sumD = _point_add u1D u2D in 
-	   let pointNorm = _norm sumD in 
-	   let (xResult, yResult, zResult) = pointNorm in 
-	   state == not(Hacl.Spec.P256.isPointAtInfinity pointNorm) /\
-	   as_nat h1 xBuffer == xResult
-    )
-)
-
-let ecdsa_verification_core publicKeyBuffer hashAsFelem r s mLen m xBuffer tempBuffer = 
-    push_frame();
-      let tempBufferU8 = create (size 64) (u8 0) in 
-      let bufferU1 =  sub tempBufferU8 (size 0) (size 32) in 
-      let bufferU2 = sub tempBufferU8 (size 32) (size 32) in 
-
-   ecdsa_verification_step23 mLen m hashAsFelem;
-   ecdsa_verification_step4 r s hashAsFelem bufferU1 bufferU2;
-   let r = ecdsa_verification_step5 publicKeyBuffer bufferU1 bufferU2 tempBuffer xBuffer in 
-   pop_frame();
-   r
-
-
-
-#reset-options "--z3refresh --z3rlimit 500"
 
 let ecdsa_verification pubKey r s mLen m = 
   push_frame();
     let tempBufferU64 = create (size 120) (u64 0) in 
-    
+    let tempBufferU8 = create (size 64) (u8 0) in 
+
     let publicKeyBuffer = sub tempBufferU64 (size 0) (size 12) in 
     let hashAsFelem = sub tempBufferU64 (size 12) (size 4) in 
     let tempBuffer = sub tempBufferU64 (size 16) (size 100) in 
 
+    let bufferU1 =  sub tempBufferU8 (size 0) (size 32) in 
+    let bufferU2 = sub tempBufferU8 (size 32) (size 32) in 
     let xBuffer =  sub tempBufferU64 (size 116) (size 4) in 
-      let h0 = ST.get() in 
 
-    bufferToJac pubKey publicKeyBuffer;
-    let publicKeyCorrect = verifyQValidCurvePoint publicKeyBuffer tempBuffer in
-    if publicKeyCorrect = false then   begin  pop_frame(); false end else 
-    let step1 = ecdsa_verification_step1 r s in  if step1 = false then begin pop_frame(); false  end 
+    let publicKeyCorrect = verifyQValidCurvePoint pubKey publicKeyBuffer tempBuffer in 
+    if publicKeyCorrect = false then 
+      begin pop_frame(); false end
     else 
-      let state = ecdsa_verification_core publicKeyBuffer hashAsFelem r s mLen m xBuffer tempBuffer in 
-      let h2 = ST.get() in 
-      assert( 
-	  let pubKeyX = as_nat h0 (gsub pubKey (size 0) (size 4)) in 
-	  let pubKeyY = as_nat h0 (gsub pubKey (size 4) (size 4)) in 
-	  let pointJac = toJacobianCoordinates (pubKeyX, pubKeyY) in 
-	 let hash = Spec.Hash.hash Spec.Hash.Definitions.SHA2_256 (as_seq h0 m) in 
-	 let hashNat = felem_seq_as_nat (Hacl.Spec.ECDSA.changeEndian(Lib.ByteSequence.uints_from_bytes_be hash)) % prime_p256_order in 
-	   let u1 = (Hacl.Spec.P256.Definitions.pow (as_nat h0 s) (prime_p256_order - 2)  * hashNat) % prime_p256_order in 
-	   let u2 = (Hacl.Spec.P256.Definitions.pow (as_nat h0 s) (prime_p256_order - 2)  * (as_nat h0 r)) % prime_p256_order in 
-	   let bufferU1 = Lib.ByteSequence.uints_to_bytes_le (nat_as_seq u1) in 
-	   let bufferU2 = Lib.ByteSequence.uints_to_bytes_le (nat_as_seq u2) in 
 
-	   let basePoint = (0x6B17D1F2E12C4247F8BCE6E563A440F277037D812DEB33A0F4A13945D898C296, 0x4FE342E2FE1A7F9B8EE7EB4A7C0F9E162BCE33576B315ECECBB6406837BF51F5, 1) in 
-	   let pointAtInfinity = (0, 0, 0) in 
-	
-	   let u1D, _ = montgomery_ladder_spec bufferU1 (pointAtInfinity, basePoint) in 
-	   let u2D, _ = montgomery_ladder_spec bufferU2 (pointAtInfinity, pointJac) in 
-	   let sumD = _point_add u1D u2D in 
-	   let pointNorm = _norm sumD in 
-	   let (xResult, yResult, zResult) = pointNorm in 
-	   state == not(Hacl.Spec.P256.isPointAtInfinity pointNorm) /\
-	   as_nat h2 xBuffer == xResult); 
-      if state = false then begin pop_frame(); false end else
-      begin 
-      let result = compare_felem_bool xBuffer r in 
-      pop_frame();
-      result
-      end
-    
+    let step1 = ecdsa_verification_step1 r s in 
+    if step1 = false then 
+      begin
+	pop_frame(); false 
+      end 
+      else 
+	begin 
+	  ecdsa_verification_step23 mLen m hashAsFelem;
+	  ecdsa_verification_step4 r s hashAsFelem bufferU1 bufferU2;
+	  let state = ecdsa_verification_step5 publicKeyBuffer bufferU1 bufferU2 tempBuffer xBuffer in 
+	    if state = false then begin pop_frame(); false end else begin
+	  let r = compare_felem xBuffer r in 
+	  pop_frame();
+	  r
+	  end
+	end   
+   
    
