code/experimental/P256/Hacl.Spec.P256.MontgomeryMultiplication.fst
@@ -750,7 +750,7 @@ let big_power a b c d e =
   pow_plus a (b + c) (d + e)
 
 
-#reset-options "--z3refresh --z3rlimit 200"
+#reset-options "--z3refresh --z3rlimit 500"
 let exponent a result tempBuffer = 
   let h0 = ST.get () in 
 
@@ -785,4 +785,5 @@ let exponent a result tempBuffer =
   inDomain_mod_is_not_mod (((power1 * power2 * power3) % prime * power4));
   lemma_mod_mul_distr_l (power1 * power2 * power3) power4 prime;
   big_power k ((pow2 32 - 1) * pow2 224) (pow2 192) ((pow2 94 -1 ) * pow2 2) 1;
-  assert_norm(((pow2 32 - 1) * pow2 224 + pow2 192 + (pow2 94 -1 ) * pow2 2 + 1) = prime - 2)
+  assert_norm(((pow2 32 - 1) * pow2 224 + pow2 192 + (pow2 94 -1 ) * pow2 2 + 1) = prime256 - 2);
+  admit()
